\documentclass[10pt,aspectratio=169]{beamer}

% All the boilerplate is in deslides.sty
\usepackage{deslides}

\author{Ji\v{r}\'i Lebl}

\institute[OSU]{%
Oklahoma State University%
%Departemento pri Matematiko de Oklahoma {\^S}tata Universitato%
}

\title{8. Substitution\\(Notes on Diffy Qs, 1.5)}

\date{}

\begin{document}

\begin{frame}
\titlepage

%\bigskip

\begin{center}
The textbook: \url{https://www.jirka.org/diffyqs/}
\end{center}
\end{frame}

\begin{frame}
As for integrals, one can use substitution for differential equations.

\medskip
\pause

\textbf{Example:}~$y' = {(x-y+1)}^2$~ is not separable nor linear.

\medskip
\pause

Let $v = x-y+1$
\pause
\quad
($v$ is a function of $x$)
\qquad
\pause
Differentiate: ~$v' = 1 - y'$
\pause
\wthus
$y' = 1-v'$

\medskip
\pause

$y' = {(x-y+1)}^2$
\wthus
$1-v' = v^2$
\pause
\wthus
$v' = 1-v^2$
\quad
\pause
(separable!)

\medskip
\pause

$\displaystyle
\frac{1}{1-v^2} \,dv = dx$
\pause
\wthus
$\displaystyle
\frac{1}{2} \ln \left\lvert  \frac{v+1}{v-1} \right\rvert = x + C$
\pause
\wthus
$\displaystyle
\left\lvert \frac{v+1}{v-1} \right\rvert = e^{2x + 2C}$
\pause
\wthus
$\displaystyle
\frac{v+1}{v-1} = D e^{2x}$

\medskip
\pause

Don't forget the singular solutions: $v=1$ and $v=-1$.

\medskip
\pause

``Unsubstitute'':

\medskip
\pause

$v=1$
\pause
\wthus
$x-y+1=1$
\pause
\wthus $y=x$
\pause
\hfill
$v=-1$
\pause
\wthus
$x-y+1=-1$
\pause
\wthus
$y=x+2$.

\medskip
\pause

$\displaystyle
\frac{v+1}{v-1} = D e^{2x}$
\pause
\wthus
$\displaystyle
\frac{x-y+2}{x-y} = D e^{2x}$
\pause
\wthus
$x-y+2 = (x-y)D e^{2x}$

\medskip

\pause
\wthus
$x-y+2 = Dx e^{2x}-yD e^{2x}$
\pause
\wthus
$-y + yD e^{2x} = Dx e^{2x} - x - 2$

\medskip

\pause
\wthus
$y\,(-1+ D e^{2x}) = Dx e^{2x} - x - 2$
\pause
\wthus
$y  = \dfrac{Dx e^{2x} - x - 2}{D e^{2x}-1}$

\medskip
\pause

Note: $D=0$ gives $y=x+2$, but no $D$ gives $y=x$.

\end{frame}

\begin{frame}

Substitution in differential equations
is the same idea as for integrals.  You guess.

\medskip
\pause

Some patterns to look for:

\begin{center}
\begin{tabular}{@{}ll@{}}
\toprule
When you see & Try substituting \\
\midrule
$yy'$ & $v=y^2$ \\
$y^2y'$ & $v=y^3$ \\
$(\cos y)y'$ & $v=\sin y$ \\
$(\sin y)y'$ & $v=\cos y$ \\
$y'e^y$ & $v=e^y$ \\ \bottomrule
\end{tabular}
\end{center}

\pause

Try to substitute in the ``most complicated'' part.

\medskip
\pause

Nothing wrong with making many guesses.

\end{frame}

\begin{frame}
\emph{Bernoulli equations}:
\quad $y' + p(x)y = q(x)y^n$.

\medskip
\pause

If $n=0$ or $n=1$ \wthus linear, we can solve.

\medskip
\pause

Otherwise $v=y^{1-n}$ will result in a linear eq.

\medskip
\pause

\textbf{Example:}
Solve
\quad
$xy'+ y(x+1)+xy^5 = 0$, \qquad $y(1)=1$.

\medskip
\pause

Note: $p(x) = (x+1)/x$ and $q(x) = -1$. \qquad (eq. is $y' + \frac{x+1}{x} \, y =
-y^5$)

\medskip
\pause

Substitute
$v=y^{1-5} = y^{-4}$
\pause
\wthus
$v' = -4 y^{-5} y'$
\pause
\wthus
$\left( \nicefrac{-1}{4} \right) y^5 v' = y'$

\medskip
\pause

$xy'+ y(x+1)+xy^5 = 0$
\pause
\wthus
$\dfrac{-xy^5}{4} v'+ y(x+1)+xy^5 = 0$
\pause
\wthus
$\dfrac{-x}{4} v'+ y^{-4}(x+1)+x = 0$

\medskip

\pause
\wthus
$\dfrac{-x}{4} v'+ v(x+1)+x = 0$
\pause
\wthus
$v'- \dfrac{4(x+1)}{x} v  = 4$
\pause
\quad (linear!)

\medskip
\pause

We just need to solve this linear equation.

\end{frame}

\begin{frame}

$v'- \frac{4(x+1)}{x} v  = 4$
\quad
($v' + P(x) v = F(x)$ where $P(x) = - \frac{4(x+1)}{x}$ and $F(x) = 4$)

\medskip
\pause

$y(1) = 1$ \wthus $v(1) = {(y(1))}^{-4} = 1$

\medskip
\pause

Assume $x > 0$ (OK as initial condition is where $x = 1$)

\medskip
\pause

Solution is:
\qquad
$\displaystyle
v(x) = e^{-\int_1^x P(s) \, ds} \left(
\int_1^x 
e^{\int_1^t P(s) \, ds}
F(t) \, dt
+
1 \right)$

\medskip
\pause

$\displaystyle
e^{\int_1^x P(s)\,ds}
\pause
= \exp \left( \int_1^x \frac{-4(s+1)}{s} \,ds \right)
\pause
=
e^{-4x-4\ln(x)+4}
\pause
= 
e^{-4x+4} x^{-4}
\pause
=
\frac{e^{-4x+4}}{x^4}$

\medskip
\pause

$\displaystyle
e^{-\int_1^x P(s)\,ds}
\pause
=
e^{4x+4\ln(x)-4}
= 
e^{4x-4} x^4$

\medskip
\pause

\thus \quad
$\displaystyle
v(x)
=
%e^{-\int_{1}^x p(s)\, ds} \left( \int_{1}^x e^{\int_{1}^t p(s)\, ds} 4 \,dt
%+ 1 \right) \\
%=
e^{4x-4} x^4
\left( \int_{1}^x 4 \frac{e^{-4t+4}}{t^4} \,dt
+ 1 \right)$
\qquad
\pause
(no closed form expression, that's OK)

\medskip
\pause

Unsubstitute:
\medskip

\quad
$y^{-4} = v$
\pause
\wthus
$\displaystyle
y = v^{-1/4}
\pause
= \frac{e^{-x+1}}{x {\left( 4 \int_1^x \frac{e^{-4t+4}}{t^4} \,dt + 1\right)}^{1/4}}$

\end{frame}

\begin{frame}

\emph{Homogeneous equations}:
\quad
$y' = F\left(\frac{y}{x}\right)$
\pause
\quad
Try
$v = \frac{y}{x}$
\pause
\qquad
$y' = v + x v'$

\medskip
\pause

$y' = F\left(\frac{y}{x}\right)$
\wthus
$v+ xv' = F(v)$
\pause
\wthus
$xv' = F(v)-v$
\pause
\wthus
$\dfrac{v'}{F(v)-v} = \dfrac{1}{x}$

\medskip
\pause

Implicit solution:
\quad
$\displaystyle
\int \frac{1}{F(v)-v} \,dv = \ln \, \lvert x \rvert + C$

\medskip
\pause

In the solution, we assume $x > 0$ or $x < 0$ depending on the initial
condition.

\end{frame}

\begin{frame}

\textbf{Example:}
Solve 
\quad
$x^2y' = y^2+xy$, \quad $y(1)=1$.

\pause
\medskip

Write $y'= {\left(\nicefrac{y}{x}\right)}^2+\nicefrac{y}{x}$,
\quad so $F(v) = v^2+v$

\pause
\medskip

Assume $x > 0$ due to the initial condition.

\medskip
\pause

Substituting \quad $v=\nicefrac{y}{x}$ \quad as above gets \quad
$xv' = v^2+v-v = v^2$

\medskip
\pause

Solve:
\quad
$\displaystyle
\int \frac{1}{F(v)-v} \,dv =
\int \frac{1}{v^2} \,dv = \ln \, \lvert x \rvert + C$
\pause
\wthus
$\displaystyle
\frac{-1}{v} = \ln  x  + C$
\pause
\wthus
$\displaystyle
v = \frac{-1}{\ln  x  + C}$

\medskip
\pause

\wthus
$\displaystyle
\frac{y}{x} = \frac{-1}{\ln  x  + C}$
\pause
\wthus
$\displaystyle
y = \frac{-x}{\ln  x  + C}$

\medskip
\pause

$1 = y(1)
\pause
= \dfrac{-1}{\ln  1  + C}
\pause
= \dfrac{-1}{C}$
\pause
\wthus
$C = -1$

\medskip
\pause

\wthus
$\displaystyle
y = \frac{-x}{\ln  x  -1}$
\end{frame}

\end{document}
